code/experimental/Hacl.Spec.P384.Definition.fst
@@ -90,3 +90,20 @@ let as_nat12 (h: mem) (e: felem12_buffer) : GTot nat =
   let s10 = s.[10] in 
   let s11 = s.[11] in 
   as_nat_t_12 (s0, s1, s2, s3, s4, s5, s6, s7, s8, s9, s10, s11)
+
+
+noextract 
+let seq_as_nat12 (s: lseq uint64 12) : GTot nat = 
+  let s0 = s.[0] in
+  let s1 = s.[1] in
+  let s2 = s.[2] in
+  let s3 = s.[3] in
+  let s4 = s.[4] in 
+  let s5 = s.[5] in 
+  let s6 = s.[6] in
+  let s7 = s.[7] in
+  let s8 = s.[8] in
+  let s9 = s.[9] in
+  let s10 = s.[10] in 
+  let s11 = s.[11] in 
+  as_nat_t_12 (s0, s1, s2, s3, s4, s5, s6, s7, s8, s9, s10, s11)
